## Solving System of Linear Equations

When we solve a system of linear equations, one of three things could happen:
- Unique Solution
- No Solution
- Family of Solutions

##### Example-1 (Unique)

$2x_{1} + 3x_{2} = 5$             ---- $(1)$
$-x_{1}+x_{2} = 7$              ---- $(2)$

Add $2$xEq$(2)$ to Eq$(1)$

$0 + 5x_{2} = 19$              ---- $(3)$
$-x_{1}+x_{2}=7$ 

Eq$(3)$ gives us $x_{2}$  which then we can plug in Eq$(2)$ to get value of $x_{1}$

***Note:*** We write out solutions in a set of ordered pair

Solution Set: $S = \{( -\frac{16}{5} \frac{,19}{5}) \}$

--------------

##### Example-2 (No Solution)

$$
\begin{align}
x_{1}-x_{2} &= 3  \:\:\:\:\:\:\:\:(1)\\
2x_{1}-3x_{2} &= 1  \:\:\:\:\:\:\:\:(2)\\
-x_{1} + 2x_{2} &= -1 \:\:\:\:\:(3)
\end{align}
$$

Add $(-2)$x$Eq(1)$ to $Eq(2)$
$$
0-x_{2} = -5 \:\:\:\:\:\:\:\:\:(4)
$$
Add $(Eq(1)$ to $Eq(3)$
$$
0+x_{2}=2 \:\:\:\:\:\:\:\:\:\:\:\:\:(5)
$$

Now we have
$$
\begin{align}
x_{1} - x_{2} &= 3 \\
-x_{2} &= -5 \\
x_{2} &= 2
\end{align}
$$
This system has no solutions
Thus,
Solution Set: $S = \phi = \{\:\}$

----------------

##### Example-3 (Family of Solution)

$$
\begin{align}
x_{1} +x_{2} - x_{3} &= 4 \:\:\:\:\:\:\:\:(1) \\
2x_{1} - x_{2} + 3x_{3} &=1 \:\:\:\:\:\:\:\:(2)
\end{align}
$$
Add $Eq(1) \cdot (-2)$  to  $Eq(2)$
$$
\begin{align}
x_{1} + x_{2} - x_{3} &= 4 \\
0 - 3x_{2} + 5x_{3} &= -7 \:\:\:\:\:\:\:\:(3)
\end{align}
$$
Divide $Eq(3)$  by  $(-3)$
$$
\begin{align}
x_{1}+x_{2} - x_{3} &= 4 \\
x_{2} - \frac{5}{3}x_{3} &= \frac{7}{3} \:\:\:\:\:\:\:\:\:\:(4)
\end{align}
$$
Add $(-1)$ x $Eq(4)$  to  $Eq(1)$
$$
\begin{align}
x_{1}+0 + \frac{2}{3}x_{3} &= \frac{5}{3} \:\:\:\:\:\:\:\:\: (5)\\
x_{2} - \frac{5}{3}x_{3} &= \frac{7}{3} \:\:\:\:\:\:\:\:\: (4)
\end{align}
$$
Choose any value for  $x_{3}$  and solve for  $x_{1}$  and $x_{2}$

Suppose we set $x_{3}=t$  for some $t \in \mathbb{R}$.  Then we get
$$
\begin{align}
x_{1} &= \frac{5}{3} - \frac{2}{3}t  \\
x_{2} &= \frac{7}{3}+\frac{5}{3}t
\end{align}
$$
Solution Set:
$$
S = \left\{\:\left( \frac{5}{3}-\frac{2}{3}t\:, \frac{7}{3}+\frac{5}{3}t,\:t\right)\:\:\Bigg|\:\:t\in\mathbb{R}\:\right\}
$$

----------------








----

### Understanding the method:

We are given a system$(A)$ of equations. We perform some operations and create a system$(B)$.
We now check the relation between solutions of $(A)$ and $(B)$

##### Example:
>Consider the system$(A)$ : $x-1=5$
>Then we perform the operation of squaring both sides
>Thus system$(B)$ : $(x-1)^{2} = 25$
>Solution sets
>$S_{A} = \{\:6\:\}$
>$S_{B} = \{\:6,-4\:\}$

These two systems are not equivalent. Every solutions of $(A)$ must satisfy $(B)$ , but not the other way around.

But suppose there exists some other operations which allow us to obtain system$(A)$ from system$(B)$.  Then, every solution of $(B)$ is a solution of $(A)$.
So the systems equivalent

#### Example (Reversible Operation)

System $A$ :
$$
\begin{align}
x_{1} + x_{2} &= 5  \:\:\:\:\:\:\:\:(1)\\
2x_{1} - x_{2} &= 2\:\:\:\:\:\:\:\: (2)
\end{align}
$$

Operation:  Replace $Eq(1) \rightarrow Eq(1)+3\cdot Eq(2)$

System $B$ :
$$
\begin{align}
(x_{1}+x_{2}) +3\cdot(2x_{1}-x_{2}) &= 5+3\cdot(2) \:\:\:\:\:\:\:\:\:\:\:\:(3) \\
\rightarrow 7x_{1} - 2x_{2} &= 11\\
2x_{1}-x_{2} &= 2 
\end{align}
$$

>Notice that $Eq(3)$ is **implied** by $Eq(1)$ and $Eq(2)$
>In other words, any solution of $Eq(1)$ and $Eq(2)$ is a solution of $Eq(3)$
>Hence, every solution of $(A)$ is a solution of $(B)$

Operation: Replace $Eq(3) \rightarrow Eq(3)-3\cdot Eq(2)$

>Lets call this new system as System $C$
>By pervious argument, every solution of $(B)$ is a solution of $(C)$
>And we observe $(C)$ is same as $(A)$ 

Thus, System $(A)$  and System $(B)$  are equivalent, $i.e$, they have the same solution sets.

This is because we obtained $(B)$ from $(A)$ by using a ***Reversible Operation***

We earlier saw with [[1. Solving Linear Equations#Understanding the method:#Example: | Previous Example]]  that squaring is **not** a Reversible Operation

----------

### Reversible Operation:

We will only use reversible operations on systems of linear equations.

1. Replace $Eq(i) \rightarrow Eq(i) + a \cdot Eq(j)$  for some $a \in \mathbb{R}$
     Inverse:  Replace $Eq(i) \rightarrow Eq(i) + (-a)\cdot Eq(j)$

2.  Interchange $Eq(i)$  and  $Eq(j)$
	  Inverse: Interchange $Eq(i)$  and  $Eq(j)$

3. Replace $Eq(i) \rightarrow a\cdot Eq(i)$   for some  $a \neq 0$
	 Inverse: Replace $Eq(i) \rightarrow (\frac{1}{a})\cdot Eq(i)$
   
#### General Idea:

Consider the System:

$$
\begin{align}
a_{11}X_{1} + a_{12}X_{2} + \dots + a_{1n}X_{n} &= b_{1} \\
a_{21}X_{1} + a_{22}X_{2} + \dots + a_{2n}X_{n} &= b_{2} \\
\vdots \quad\qquad\qquad\qquad\qquad\qquad & \quad\:\vdots \\
a_{m1}X_{1} + a_{m2}X_{2} + \dots + a_{mn}X_{n} &= b_{m}
\end{align} 
$$
Suppose $a_{11} \neq 0$

- We replace $Eq(1) \rightarrow (\frac{1}{a}) \cdot Eq(1)$  to reduce to a situation where the coefficient of $X_{1}$ in $Eq(1)$ is $1$ 

- Now, eliminate $X_{1}$ from $Eq(2),\dots,Eq(m)$ by
  $Eq(i) \rightarrow Eq(i) + (-a_{j_{1}})\cdot Eq(1)$
  for $i = 2,3 \dots m$
$$
\begin{align}
X_{1} + c_{12}X_{2} + \dots + c_{1n}X_{n} &= d_{1} \\
0X_{1} + c_{22}X_{2} + \dots + c_{2n}X_{n} &= d_{2} \\
\vdots \quad\qquad\qquad\qquad\qquad\qquad & \quad\:\vdots \\
0X_{1} + c_{m2}X_{2} + \dots + c_{mn}X_{n} &= d_{m}
\end{align} 
$$

- Now consider a **New System** from $Eq(2)$ to $Eq(m)$ with $(n-1)$ variables and $(m-1)$ equations
  Solve this **New System** for $X_{2}\dots X_{n}$ and substitute in $Eq(1)$. 
  Solve $Eq(1)$ for $X_{1}$

> If $a_{11} = 0$ :
> Find some $i$ such that $a_{i1} \neq 0$
> Interchange $Eq(1)$  and  $Eq(i)$
> If $a_{i1} = 0$ for all $i$, then $X_{1}$ is not really there in any equation, Move on to $X_{2}$

- Repeat similar procedure with **System-2** which will end up in **System-3** with $(n-2)$ variables and $(m-2)$ equations $\dots$ and so on.

##### Example:
$$
\begin{align}
-x + y +2z +3w &= -6 \\
-5x - 2y +0z + 11w &= -27 \\
-2x +0y +z + 5w &= -11
\end{align}
$$
Multiply $Eq(1)$ by $(-1)$

$Eq(2) \rightarrow Eq(2) + 5\cdot Eq(1)$
$Eq(3) \rightarrow Eq(3) + 2\cdot Eq(1)$

$$
\begin{align}
x  - y -2z -3w &= 6 \\
-7y - 10z -4w &= 3  \\
-2y - 3z - w &= 1
\end{align}
$$
$Eq(2) \rightarrow -\frac{1}{7} \cdot Eq(2)$
$Eq(3) \rightarrow Eq(3) +2\cdot Eq(2)$


