#### Expansion

***By Rows:***
> Let $1 \leq k \leq n$ 
> Then, 
> 	$\det(A) = \sum_{l=1}^{n}(-1)^{k+l}\cdot a_{kl}\cdot \det(A_{kl})$

***By Columns:***
> Let $1 \leq k \leq n$ 
> Then, 
> 	$\det(A) = \sum^{n}_{l=1}(-1)^{k+l} \cdot a_{lk}\cdot \det(A_{lk})$

##### Example (can skip its just calculating determinants)
$$
A = \begin{pmatrix}
1 & 0 & 2 \\
4 & -1 & 5 \\
2 & 6 & 8
\end{pmatrix}
$$
We will expand along the first column
$$
\begin{align}
A_{11} = \begin{pmatrix}
-1 & 5 \\
6 & 8
\end{pmatrix}
,\quad A_{21} &= \begin{pmatrix}
0 & 2 \\
6 & 8
\end{pmatrix}
, \quad A_{31} = \begin{pmatrix}
0 & 2 \\
-1 & 5
\end{pmatrix} \\ \\
\det(A) &= (-1)^{1+1}\cdot 1 \cdot \det \begin{pmatrix}
-1 & 5 \\
6 & 8
\end{pmatrix} \\ \\
&\quad+ (-1)^{2+1}\cdot 4 \cdot \det \begin{pmatrix}
0 & 2 \\
6 & 8
\end{pmatrix} \\  \\
&\quad+ (-1)^{3+1}\cdot 2 \cdot \det \begin{pmatrix}
0 & 2 \\
-1 & 5
\end{pmatrix}


\end{align}


$$
Each of the $2$x$2$ matrices can be calculated similarly
Like,
$$
\begin{align}
\det \left(\begin{array}
--1 & 5 \\
6 & 8
\end{array}\right) &= 
(-1)^{1+1}\cdot (-1)\cdot \det(8)+(-1)^{2+1} \cdot 6 \cdot \det(5) \\ \\
&= -8 -30 = -38
\end{align}
$$
Thus we get,
	$\det(A)=1\cdot(-38)-4\cdot(-8)+2\cdot(-2) = -8$

---
### Cofactors

$C = (c_{ij})_{i,j}$
where,
	$c_{ij}=(-1)^{i+j}\det(A_{ij})$

***For 2x2 matrix***:
$$
A = \begin{pmatrix}
a & b \\
c & d
\end{pmatrix} ; \quad
A^{-1} = \begin{pmatrix}
d & -c \\
-b & a
\end{pmatrix}
$$

#### Finding Inverse by Cofactor Matrix
$$
A^{-1}= \frac{adj(A)}{\det(A)}
$$
where,
$$
adj(A) = C^{T}
$$


---
### Properties of Determinants

1. Let $B$ be obtained from $A$ by performing an elementary row operation.
   - If the operation is $R_{i}+xR_{j}$
     Then $\color{#fc6f86}\det(B) = \det(A)\:\:;\:\:(i \neq j)$
   - If the operation is $R_{i} \leftrightarrow R_{j} \:\:(i \neq j)$
     Then, $\color{#fc6f86}\det(B) = -\det(A)$
   - If the operation is $xR_{i}\:\:\:(x \neq 0)$, 
     Then, $\color{#fc6f86}\det(B)=x\det(A)$

2. Similar formulas hold for column operations, which we denote by $C_{i}+xC_{j}$, etc...
   
3. $\det(I_{n})=1$  for any $n$

4. $\det(AB)=\det(A) \cdot \det(B)$   for any $A,B \in M_{n\text{x}n}(\mathbb{R})$ 

---

### Transpose of a Matrix

Let, $A$ be a matrix then, $A^{T}$ is the ***Transpose*** of $A$
$$
A = \begin{pmatrix}
a & b \\
c & d
\end{pmatrix};
\quad
A^{T} = \begin{pmatrix}
a & c \\
b & d
\end{pmatrix}

$$
Also,
	$\det(A^{T}) = \det(A)$

We will now see that the Transpose is not just exchanging rows and columns

I will use the concepts of **Linear Transformations** which is not covered yet but I would like to cover the transpose here so deal with it.

Refer to this video for explanation of **Linear Transformation**

<iframe title="Linear transformations and matrices | Chapter 3, Essence of linear algebra" src="https://www.youtube.com/embed/kYB8IZa5AuE?feature=oembed" height="113" width="200" allowfullscreen="" allow="fullscreen" style="aspect-ratio: 1.76991 / 1; width: 100%; height: 100%;"></iframe>

A transpose will always try to recover the original form of the matrix while preserving its measurements when a linear transformation is applied to it.
You can say a Transpose is kind of a Inverse.

![](https://i.imgur.com/izsKKYI.gif)

If any linear transformation doesn't change the lengths of the unit vectors, i.e., in case of a rotation. then the transpose becomes an Inverse
	i.e.,
	***Orthogonal Matrix***: $A^{T} = A^{-1}$

---

```ad-note
title: Note
If $Row(i)$ and $Row(j)$ of a matrix $A$ are identitcal.

Then, the operation $R_{i} + (-1)R_{j}$ turns the $i^{th}$ row into a row of zeroes

Expanding along this row, we get $\det(A) = 0$

Thus if any two Rows of a det are identitcal its value is 0
```


#### Theorem
A square matrix $A$ is invertible $\iff$ $\det(A) \neq 0$
If $\det(A) \neq 0$
	$\color{#d693f5}A^{-1}=\det(A)^{-1} \cdot C^{tr}$
where $C =$ cofactor matrix of A

###### Proof:
> ~

---

## Cramer's Rule

Suppose we have a system of n linear equations in the n variables $X_{1},X_{2}\dots X_{n}$
$$
\begin{align}
a_{11}X_{1} + a_{12}X_{2} + \dots + a_{1n}X_{n} &= b_{1} \\
a_{21}X_{1} + a_{22}X_{2} + \dots + a_{2n}X_{n} &= b_{2} \\
\vdots \quad\qquad\qquad\qquad\qquad\qquad & \quad\:\vdots \\
a_{m1}X_{1} + a_{m2}X_{2} + \dots + a_{mn}X_{n} &= b_{m}
\end{align} 
$$
As usual, we write this using matrices
$$
A = (a_{ij})_{i,j} \:\:\:; \quad X= \begin{pmatrix}
X_{1} \\
\vdots \\
X_{n}
\end{pmatrix}
\:\:\:; \quad 
B = \begin{pmatrix}
b_{1} \\
\vdots \\
b_{n}
\end{pmatrix}
$$
We want to solve the matrix equation $AX=B$
$X=A^{-1}B$      (if $A$ is invertible)
$X = \left( \frac{1}{\det(A)} \right) \cdot C^{T} \cdot B$

##### Defining $D_{x_{n}}$ 
Interchange any column of $A$ with the column matrix $B$ 

***Example:***
> $$
\begin{align}
A = \begin{pmatrix}
1 & 2 & 3 \\
4 & 5 & 6 \\
7 & 8 & 9
\end{pmatrix} \quad
B &= \begin{pmatrix}
-1 \\
-2 \\
-3
\end{pmatrix} \quad 
X = \begin{pmatrix}
x \\
y \\
z
\end{pmatrix} \\  \\
D_{x} = \begin{pmatrix}
-1 & 2 & 3 \\
-2 & 5 & 6 \\
-3 & 8 & 9
\end{pmatrix}
\quad D_{y} &= \begin{pmatrix}
1 & -1 & 3 \\
4 & -2 & 6 \\
7 & -3 & 9
\end{pmatrix}
\quad D_{z} = \begin{pmatrix}
1 & 2 & -1 \\
4 & 5 & -2 \\
7 & 8 & -3
\end{pmatrix}


\end{align}
$$

***To find the solutions:***
> $x = \frac{D_{x}}{D},\:\:y = \frac{D_{y}}{D},\:\: z = \frac{D_{z}}{D}$

---



