## Products of Inertia

$$
\require{physics}
<<<<<<< HEAD
I_{xx} = \Sigma m_{j}(y_{j}^{2}+)
$$
=======
\begin{align}
I_{xx} &= \Sigma m_{j}(y_{j}^{2}+z_{j}^{2}) \\ 
I_{yy} &= \Sigma m_{j}(x_{j}^{2}+z_{j}^{2}) \\
I_{zz} &= \Sigma m_{j}(x_{j}^{2}+y_{j}^{2}) \\ \\
I_{xy} &= - \Sigma m_{j}x_{j}y_{j}  \\
I_{xy} &= - \Sigma m_{j}x_{j}y_{j}  \\
I_{xy} &= - \Sigma m_{j}x_{j}y_{j}  \\ \\
I_{xy} &= - \Sigma m_{j}x_{j}y_{j}  \\
I_{xy} &= - \Sigma m_{j}x_{j}y_{j}  \\
I_{xy} &= - \Sigma m_{j}x_{j}y_{j} 
\end{align}
$$
>>>>>>> origin/main
