Recall the Cosets of $m\mathbb{Z}$ are $m\mathbb{Z}, 1+m\mathbb{Z} , \dots (m+1)+m\mathbb{Z}$
For Integers (i.e., $\mathbb{Z}$)
	1. $a+m\mathbb{Z} = b+m\mathbb{Z}$
	2. $a-b$ is divisible by $m$
	3. $a$ and $b$ leave the same remainder when divided by $m$

##### Notation: Mod m

$$a \equiv b \: \: \:(mod \: m )$$
if $m$ divideds $a-b$.
Read as: "$a$ is congruent to $b$ modulo $m$"
meaning $a$ and $b$ are in the same coset of $m\mathbb{Z}$

-------------------------------------

### Arithmetics of mod m

#### Addition:
$$a+c\equiv b+d \: \: \: \: (mod \: \: \: m)$$
***Proof:***
>	$a-b\equiv mx$    &    $c-d \equiv my$ 
>	($x,y \in \mathbb{Z}$)
$$
\begin{align}
(a+c)-(b+d)&=(a-b)+(c-d) \\
&=mx+my \\
&=m(x+y)
\end{align}
$$
>So, $a+c \equiv b+d$  $(mod \: \: m)$


#### Multiplication:
$$
ac \equiv bd \:\:\:\:\:\:\:(mod \: \: \: m)
$$
Same Proof as before

*Thus we can define binary operations + and * on $\mathbb{Z}/m\mathbb{Z}$

-----------------------------
### Binary Operations on $\mathbb{Z}/m\mathbb{Z}$

$(\mathbb{Z}/m\mathbb{Z}, +)$ is a group

***Identity***
   >$m\mathbb{Z}$ is the identity. Indeed 
   >$(m\mathbb{Z})+(a+m\mathbb{Z})$ = $(0+a)+m\mathbb{Z} = a+m\mathbb{Z}$
   >Similarly,
   >	$(a+m\mathbb{Z})+(m\mathbb{Z})= (a+m\mathbb{Z})$
   
Take $a=1$ and add $a=0$ getting the set back 
![[Pasted image 20221204141901.png]]

***Inverses***
>$(a+m\mathbb{Z})+((-a)+m\mathbb{Z})$
>$=(a+(-a))+m\mathbb{Z}$
>$=m\mathbb{Z}$

***Associativity***
$$
\begin{align}
(a+m\mathbb{Z})+(b+m\mathbb{Z})+(c+m\mathbb{Z})&=(a+(b+c))+m\mathbb{Z} \\
&=((a+b)+c)+m\mathbb{Z} \\
&=((a+m\mathbb{Z})+(b+m\mathbb{Z}))+(c+m\mathbb{Z})
\end{align}
$$


Is $(\mathbb{Z}/m\mathbb{Z},*)$ a group?
Here
	$(1+m\mathbb{Z})$ is the identity for Multiplication
	Its also Associative.
***Though its not a group under multiplication***

-------------------------------------------------

### Multiplicative Inverses in $\mathbb{Z}/m\mathbb{Z}$

We say that an element $(a+m\mathbb{Z})$ on $(\mathbb{Z}/m\mathbb{Z})$ is **Invertible** if it has a multplicative inverse 
i.e,
	$(a+m\mathbb{Z})\cdot(b+m\mathbb{Z})=1+m \mathbb{Z}$

Suppose $a+m\mathbb{Z}$ has a multplicative inverse $b+m\mathbb{Z}$
Then
	$ab=m\mathbb{Z}=1+m\mathbb{Z}$
	$\implies ab\equiv 1 \: \: (mod \: \: m)$
Thus $m \: |  \: ab-1$
Let $d$ be any common factor of $m$ and $a$
Thus $m=dx$ and $a=dy$  for some $x,y \in \mathbb{Z}$
As, 
	$m \: | \: ab-1$   ,   $ab-1=mz$   for some $z \in \mathbb{Z}$
So,
$$
\begin{align}
1&=ab-mz \\
&=(dy)b-(dx)z \\
&=d(yb-xz)
\end{align}
$$
So, $d \: | \: 1 \implies d=-+1$

```ad-note
title: Conclusion
$a+m\mathbb(Z)$ is invertible only if gcd$(a,m)=1$ , i.e, $a$ and $m$ are coprime
```


#### Lemma 1

```ad-note
title: Lemma-1
Let $m \in \mathbb{Z}, \: \:m>0$
If $gdc(a,m)=1$ , then for any element $x \in a+m\mathbb{Z}$ , we have $gcd(x,m)=1$
```

***Proof:***
> Let $d$ be a common factor of $x$ and $m$. So, $x=dr$ and $x=ds$, For some $r,x \in \mathbb{Z}$
> As $x \in a+m\mathbb{Z} \rightarrow x=a+mt$   for some $t\in\mathbb{Z}$
> So, $dr=a+dst \rightarrow a=d(r-st)$
> So, $d\:|\:a$ 
> Also, $d\:|\:m$
> Thus $gcd(a,m)=1 \implies d=\pm 1$ 
> Thus $gcd(x,m)=1$

----------------------------------------

### Unitary Group

The set of all elements of $\mathbb{Z}/m\mathbb{Z}$  coprime to $m$ is denoted by $U(m)$.

***Note**
> $1+m\mathbb{Z}$ is in $U(m)$ if $m>1$

##### Notation:
Thus 
	We can write the elements $a+m\mathbb{Z}$ of $\mathbb{Z}/m\mathbb{Z}$ as $\bar{a}$ 
	Thus,
		$\mathbb{Z}/m\mathbb{Z}=\{\bar{0}, \bar{1}, \bar{2}\dots,\overline{(m-1)}$

---------------------------

#### Lemma 2

If $a,b$ are intergers such that $\bar{a}, \bar{b} \in U(m)$  , then $\overline{ab} \in U(m)$

***Proof:***
> $a\equiv 1 \: (mod \: m )$
> $b \equiv 1 \: (mod \: m)$
> $a-1=mx$    &    $b-1=my$
> $ab-1=(mx-1)(my-1)-1$
> $ab-1=m(mxy-x-y)$
> Thus 
> 	$m \: | \: ab-1$
> $ab \equiv 1 \: (mod \: \: m)$


----------------------------------

#### Lemma 3

Let $\bar{a},\bar{x},\bar{y} \in \mathbb{Z}/m\mathbb{Z}$
Suppose  $\bar{a}\in U(m)$
If $\bar{a}\bar{x}=\bar{a}\bar{y}$ , then  $\bar{x}=\bar{y}$

***Proof***
>  $\bar{a}\bar{x}=\bar{a}\bar{y} \implies m \: | \: a(x-y)$
>  And $gcd(a,m)=1 \implies m \: | \: x-y \implies \bar{x}=\bar{y}$

-------------------------------
#### Theorem:

Let $m$ be a positive integer. If $\bar{a} \in U(m)$ , there exists $\bar{b}$ in $U(m)$ such that $\bar{a}\cdot  \bar{b} = \bar{1}$

***Proof:***
> Let $\phi: \: U(m) \rightarrow U(m)$
> $\phi(\bar{x}) = \bar{a}\cdot  \bar{x}$                  (Lemma 2 $\implies  \bar{a}\cdot  \bar{x} \in U(m)$)
> Thus $\phi$ is a bijection
> Such that $\bar{b} \in U(m) \implies \phi(\bar{b}) = \bar{1}$
> So, $\bar{a}  \bar{b} = \bar{1}$

**Collorary:** $U(m)$ is a group under multiplication

***Example***
>1. $m=6$
>   $U(6) = \{\bar{1} , \bar{5}\}$
>   Note: $\bar{5}^2 = \overline{25} = \bar{1}$
> 2. $m=10$
>    $U(10) = \{ \bar{1} , \bar{3} , \bar{7} , \bar{9}\}$
>    $\bar{3}^{2} = \bar{9} \: \: \: , \: \: \: \bar{3}^{3} = \overline{27} = \bar{7}$


--------------------------------------------

